\documentclass{article}
\usepackage[english]{babel}
\usepackage{amsfonts}
%\usepackage{a4wide}
\usepackage{setspace}
\usepackage{amsmath}
\usepackage{amsfonts}
\usepackage{amssymb,enumerate}
\usepackage{amsthm,stmaryrd}
\usepackage[all]{xy}
\usepackage{hyperref}

\newcommand{\lls}{\mathcal{S}}
\newcommand{\bbp}{\mathbb{P}}

\textwidth 6.0in \oddsidemargin 0.0in

\begin{document}

\vspace{3 mm}

\noindent \textbf{Problem 3} (Jacod and Protter, pg. 46 Problem 7.17) Suppose a distribution function $F$ is given by
\begin{eqnarray*} F(x) = \frac{1}{4}\mathbf{1}_{[0, \infty)}(x) + \frac{1}{2}\mathbf{1}_{[1,\infty)}(x) + \frac{1}{4}\mathbf{1}_{[2,\infty)}(x). \end{eqnarray*}  Let $\mathbb{P}$ be given by
		\begin{eqnarray*} \mathbb{P}((-\infty, x]) = F(x), ~~~~~~~ x \in \mathbb{R}. \end{eqnarray*}  Find the probabilities of the following events:  $A = (-1/2, 1/2)$; $B = (-1/2, 3/2)$; $C = (2/3, 5/2)$; $D = [0,2)$; $E = (3,\infty)$.

\vspace{2 mm}
\noindent \textbf{Solution.}\\
Based on the Corollary 7.1 from Jacod\rq s textbook, 
\begin{enumerate}[(1)]
	\item 
		$$\bbp(A) = \bbp((-1/2,1/2)) = F((1/2)^-) - F(-1/2).$$
		\begin{align*}
		F((1/2)^-) &=  \frac{1}{4}\mathbf{1}_{[0, \infty)}((1/2)^-) + \frac{1}{2}\mathbf{1}_{[1,\infty)}((1/2)^-) + \frac{1}{4}\mathbf{1}_{[2,\infty)}((1/2)^-) \\
				 &	= 1/4+ 0+ 0  = 1/4,
		\end{align*}
		and
		\begin{align*}
        F(-1/2) &=  \frac{1}{4}\mathbf{1}_{[0, \infty)}(-1/2) + \frac{1}{2}\mathbf{1}_{[1,\infty)}(-1/2) + \frac{1}{4}\mathbf{1}_{[2,\infty)}(-1/2) \\
        			 &= 0 + 0 + 0 = 0.
        \end{align*}
        So
        $$\bbp(A) = 1/4 - 0 = 1/4.$$
	\item
		$$\bbp(B) = \bbp((-1/2,3/2)) = F((3/2)^-) - F(-1/2).$$
		\begin{align*}
		F((3/2)^-) &=  \frac{1}{4}\mathbf{1}_{[0, \infty)}((3/2)^-) + \frac{1}{2}\mathbf{1}_{[1,\infty)}((3/2)^-) + \frac{1}{4}\mathbf{1}_{[2,\infty)}((3/2)^-)- \\
			       &= 1/4+ 1/2+ 0  = 3/4,
		\end{align*}
		and
		\begin{align*}
        	F(-1/2) &=  \frac{1}{4}\mathbf{1}_{[0, \infty)}(-1/2) + \frac{1}{2}\mathbf{1}_{[1,\infty)}(-1/2) + \frac{1}{4}\mathbf{1}_{[2,\infty)}(-1/2) \\
        			&= 0 + 0 + 0 = 0.
        \end{align*}
        So
        $$\bbp(B) = 3/4 - 0 = 3/4.$$
	\item
		$$\bbp(C) = \bbp((3/2,5/2)) = F((5/2)^-) - F(3/2).$$
		\begin{align*}
			F((5/2)^-) &=  \frac{1}{4}\mathbf{1}_{[0, \infty)}((5/2)^-) + \frac{1}{2}\mathbf{1}_{[1,\infty)}((5/2)^-) + \frac{1}{4}\mathbf{1}_{[2,\infty)}((5/2)^-) \\
					   &= 1/4+ 1/2+ 1/4  = 1,
		\end{align*}
		and
		\begin{align*}
        	F(3/2) &=  \frac{1}{4}\mathbf{1}_{[0, \infty)}(3/2) + \frac{1}{2}\mathbf{1}_{[1,\infty)}(3/2) + \frac{1}{4}\mathbf{1}_{[2,\infty)}(3/2) \\
        		   &= 1/4 + 1/2 + 0 = 3/4.
        \end{align*}
        So
        $$\bbp(C) = 1 - 3/4 = 1/4.$$
	\item
		$$\bbp(D) = \bbp([0,2)) = F(2^-) - F(0^-).$$
		\begin{align*}
			F(2^-) &=  \frac{1}{4}\mathbf{1}_{[0, \infty)}(2^-) + \frac{1}{2}\mathbf{1}_{[1,\infty)}(2^-) + \frac{1}{4}\mathbf{1}_{[2,\infty)}(2^-) \\
				   &= 1/4+ 1/2+ 0  = 3/4,
		\end{align*}
		and
		\begin{align*}
        	F(0^-) &=  \frac{1}{4}\mathbf{1}_{[0, \infty)}(0^-) + \frac{1}{2}\mathbf{1}_{[1,\infty)}(0^-) + \frac{1}{4}\mathbf{1}_{[2,\infty)}(0^-) \\
        		   &= 0 + 0 + 0 = 0.
        \end{align*}
        So
        $$\bbp(D) = 3/4 - 0 =3/4.$$
	\item
		$$\bbp(E) = \bbp((3,\infty)) = F(\infty) - F(3) = 1 - F(3).$$
		$$F(3) \geq F(5/2) = 1,$$ since $F$ is monotone increasing and
		$$F(3) \leq 1$$ since $0\leq F(x) \leq 1, x \in R$.\\
		So $$F(3) = 1.$$
		Thus $$\bbp(E) = 1 - F(3) = 0.$$

\end{enumerate}	


\end{document}

